
          %%%%% ~~~~~~~~~~~~~~~~~~~~ %%%%%

\section{Maxwell's equations -- gauge theory, gauge field}
\setcounter{theorem}{0}
\setcounter{equation}{0}

%\renewcommand{\theenumi}{\alph{enumi}}
%\renewcommand{\labelenumi}{\textnormal{(\theenumi)}$\;\;$}
\renewcommand{\theenumi}{\roman{enumi}}
\renewcommand{\labelenumi}{\textnormal{(\theenumi)}$\;\;$}

          %%%%% ~~~~~~~~~~~~~~~~~~~~ %%%%%

\begin{theorem}[Gauge field gives rise to electric, magnetic fields that satisfy Maxwell's equations]
\mbox{}
\vskip 0.2cm
\noindent
Suppose:
\begin{itemize}
\item
	$U \subset \Re^{1,3}$ is an open subset.
\item
	\,$\rho, J^{1}, J^{2}, J^{3}, A_{0}, A_{1}, A_{2}, A_{3}$\,
	are smooth \,$\Re$-valued functions defined on $U \subset \Re^{1,3}$.
\end{itemize}
\vskip 0.3cm
\noindent
Define the following $3$-vectors:
\begin{eqnarray*}
J
& := &
	J_{1}\,\dfrac{\partial}{\partial x^{1}} \,+\, J_{2}\,\dfrac{\partial}{\partial x^{2}} \,+\, J_{3}\,\dfrac{\partial}{\partial x^{3}}
\\
\overset{{\color{white}\textnormal{\Large$1$}}}{A}
& := &
	A_{1}\,\dfrac{\partial}{\partial x^{1}} \,+\, A_{2}\,\dfrac{\partial}{\partial x^{2}} \,+\, A_{3}\,\dfrac{\partial}{\partial x^{3}}
\\
\overset{{\color{white}\textnormal{\Large$1$}}}{B}
& = &
	B^{1}\,\dfrac{\partial}{\partial x^{1}} \,+\, B^{2}\,\dfrac{\partial}{\partial x^{2}} \,+\, B^{3}\,\dfrac{\partial}{\partial x^{3}}
\;\; := \;\;
	\nabla \times A
\\
\overset{{\color{white}\textnormal{\Large$1$}}}{E}
& = &
	E^{1}\,\dfrac{\partial}{\partial x^{1}} \,+\, E^{2}\,\dfrac{\partial}{\partial x^{2}} \,+\, E^{3}\,\dfrac{\partial}{\partial x^{3}}
\;\; := \;\;
	\nabla A_{0} \,-\, \dfrac{\partial A}{\partial x^{0}}
\end{eqnarray*}
\vskip 0.3cm
\noindent
Define the following $1$-forms:
\begin{eqnarray*}
\mathbf{J}
& := &
	\rho \, \d x^{0} \,-\, J^{1}\,\d x^{1} \,-\, J^{2}\,\d x^{2} \,-\, J^{3}\,\d x^{3}
\\
\mathbf{A}
& := &
	A_{0}\,\d x^{0} \,+\, A_{1}\,\d x^{1}  \,+\, A_{2}\,\d x^{2}  \,+\, A_{3}\,\d x^{3}
\\
\mathbf{E}
& := &
	E^{1}\,\d x^{1} \,+\, E^{2}\,\d x^{2} \,+\, E^{3}\,\d x^{3}
\end{eqnarray*}
\vskip 0.3cm
\noindent
And, define the following $2$-forms:
\begin{eqnarray*}
\mathbf{B}
& := &
	B^{1}\;\d x^{2} \wedge \d x^{3}
	\;+\;
	B^{2}\;\d x^{3} \wedge \d x^{1}
	\;+\;
	B^{3}\;\d x^{1} \wedge \d x^{2}
\\
\mathbf{F}
& := &
	- \, \d x^{0} \wedge \mathbf{E} \, + \, \mathbf{B}
\\
& = &
	- \; E^{1}\;\d x^{0} \wedge \d x^{1} \; - \; E^{2}\;\d x^{0} \wedge \d x^{2} \; - \; E^{3}\;\d x^{0} \wedge \d x^{3}
\\
&&
	+\;
	B^{1}\;\d x^{2} \wedge \d x^{3}
	\;+\;
	B^{2}\;\d x^{3} \wedge \d x^{1}
	\;+\;
	B^{3}\;\d x^{1} \wedge \d x^{2}
\end{eqnarray*}
Then,
\begin{enumerate}
\item
	$\mathbf{F} \; = \; \d\,\mathbf{A}$.
\item
	$B$ and $E$ satisfy Gauss's law for magnetic fields (non-existence of magnetic monopoles) and Faraday's law, i.e.
	\begin{equation*}
	\nabla \bullet B \;\; = \;\; 0
	\quad\quad\textnormal{and}\quad\quad
	\dfrac{\partial B}{\partial t} \;\; = \;\; -\,\nabla \times E
	\end{equation*}	
\item	
	$B$ and $E$ satisfy Gauss's law for electric fields and Amp\`{e}re-Maxwell's law, i.e.
	\begin{equation*}
	\nabla \bullet E \;\; = \;\; 4 \pi \cdot \rho
	\quad\quad\textnormal{and}\quad\quad
	\dfrac{\partial E}{\partial t} \;\; = \;\; \nabla \times B \,-\, 4\,\pi\cdot J
	\end{equation*}
	if and only if \,$\mathbf{A}$ satisfies:
	\begin{equation*}
	\left\{\begin{array}{ccl}
		-\,\Delta A_{0} + \dfrac{\partial}{\partial x^{0}}\!\left(\,\nabla \bullet A\,\right)
		& = &
			- \, 4\,\pi\cdot\rho
		\\ \\
		\left(\,\dfrac{\partial^{2}}{\partial(x^{0})^{2}} - \Delta\,\right)A
		+
		\nabla\left(\, -\,\dfrac{\partial A_{0}}{\partial x^{0}} + \nabla \bullet A \,\right)
		& = &
			{\color{white}-} \, 4\,\pi \cdot J
		\end{array}\right.
	\end{equation*}
\end{enumerate}
\end{theorem}
\proof
\begin{enumerate}
\item
	Note that:
	\begin{equation*}
	B
	\;\; := \;\;
		\nabla \times A
	\;\; = \;\;
		\underset{B^{1}}{\underbrace{\left(\,\dfrac{\partial A_{3}}{\partial x^{2}} - \dfrac{\partial A_{2}}{\partial x^{3}}\,\right)}}
		\,\dfrac{\partial}{\partial x^{1}}
		\; + \;
		\underset{B^{2}}{\underbrace{\left(\,\dfrac{\partial A_{1}}{\partial x^{3}} - \dfrac{\partial A_{3}}{\partial x^{1}}\,\right)}}
		\,\dfrac{\partial}{\partial x^{2}}
		\; + \;
		\underset{B^{3}}{\underbrace{\left(\,\dfrac{\partial A_{2}}{\partial x^{1}} - \dfrac{\partial A_{1}}{\partial x^{2}}\,\right)}}
		\,\dfrac{\partial}{\partial x^{3}}
	\end{equation*}
	\begin{equation*}
	E
	\;\; := \;\;
		\nabla A_{0} \,-\, \dfrac{\partial A}{\partial x^{0}}
	\;\; = \;\;
		\underset{E^{1}}{\underbrace{\left(\,\dfrac{\partial A_{0}}{\partial x^{1}} - \dfrac{\partial A_{1}}{\partial x^{0}}\,\right)}}
		\,\dfrac{\partial}{\partial x^{1}}
		\; + \;
		\underset{E^{2}}{\underbrace{\left(\,\dfrac{\partial A_{0}}{\partial x^{2}} - \dfrac{\partial A_{2}}{\partial x^{0}}\,\right)}}
		\,\dfrac{\partial}{\partial x^{2}}
		\; + \;
		\underset{E^{3}}{\underbrace{\left(\,\dfrac{\partial A_{0}}{\partial x^{3}} - \dfrac{\partial A_{3}}{\partial x^{0}}\,\right)}}
		\,\dfrac{\partial}{\partial x^{3}}
	\end{equation*}
	Hence,
	\begin{eqnarray*}
	&&
		\d\,\mathbf{A}
	\;\; = \;\;
		\d\!\left(\,A_{\nu}\,\d x^{\nu}\,\right)
	\;\; = \;\;
		\dfrac{\partial A_{\nu}}{\partial x^{\mu}} \cdot \d x^{\mu} \wedge \d x^{\nu}
	\\ \\
	& = &
		\,{\color{white}+}\,
		\left(\,\dfrac{\partial A_{1}}{\partial x^{0}} - \dfrac{\partial A_{0}}{\partial x^{1}}\,\right)\d x^{0} \wedge \d x^{1}
		\,+\,
		\left(\,\dfrac{\partial A_{2}}{\partial x^{0}} - \dfrac{\partial A_{0}}{\partial x^{2}}\,\right)\d x^{0} \wedge \d x^{2}
		\,+\,
		\left(\,\dfrac{\partial A_{3}}{\partial x^{0}} - \dfrac{\partial A_{0}}{\partial x^{3}}\,\right)\d x^{0} \wedge \d x^{3}
	\\
	&&
		\,+\,
		\left(\,\dfrac{\partial A_{2}}{\partial x^{1}} - \dfrac{\partial A_{1}}{\partial x^{2}}\,\right)\d x^{1} \wedge \d x^{2}
		\,+\,
		\left(\,\dfrac{\partial A_{3}}{\partial x^{1}} - \dfrac{\partial A_{1}}{\partial x^{3}}\,\right)\d x^{1} \wedge \d x^{3}
		\,+\,
		\left(\,\dfrac{\partial A_{3}}{\partial x^{2}} - \dfrac{\partial A_{2}}{\partial x^{3}}\,\right)\d x^{2} \wedge \d x^{3}
	\\ \\
	& = &
		\,-\,
		E^{1} \cdot \d x^{0} \wedge \d x^{1}
		\,-\,
		E^{2} \cdot \d x^{0} \wedge \d x^{2}
		\,-\,
		E^{3} \cdot \d x^{0} \wedge \d x^{3}
	\\
	&&
		\,+\,
		B^{3} \cdot \d x^{1} \wedge \d x^{2}
		\,-\,
		B^{2} \cdot \d x^{1} \wedge \d x^{3}
		\,+\,
		B^{1} \cdot \d x^{2} \wedge \d x^{3}
%	\\ \\
%	& = &
%		\,-\,
%		E^{1} \cdot \d x^{0} \wedge \d x^{1}
%		\,-\,
%		E^{2} \cdot \d x^{0} \wedge \d x^{2}
%		\,-\,
%		E^{3} \cdot \d x^{0} \wedge \d x^{3}
%		\,+\,
%		B^{3} \cdot \d x^{1} \wedge \d x^{2}
%		\,+\,
%		B^{2} \cdot \d x^{3} \wedge \d x^{1}
%		\,+\,
%		B^{1} \cdot \d x^{2} \wedge \d x^{3}
	\\ \\
	& =: &
		\mathbf{F}\,,
	\end{eqnarray*}
	as required.
\item
	We just established that
	\,$\mathbf{F} \, = \, \d\,\mathbf{A}$,\,
	which in turn implies
	\,$\d\,\mathbf{F} \, = \, \d^{2}\,\mathbf{A} \, = \, 0$\,
	(since \,$\d^{2} \, = \, \d \circ \d \, = \, 0$).
	Hence, by Theorem \ref{MaxwellsEquationsDifferentialForms},
	\,$B$\, and \,$E$\, satisfy
	Gauss's law for magnetic fields (non-existence of magnetic monopoles) and Faraday's law.
\item
	First, note that
	\begin{eqnarray*}
	\d\,\mathbf{A}
	& = &
		\d\!\left(\,A_{\nu}\,\d x^{\nu}\,\right)
	\;\; = \;\;
		\dfrac{\partial A_{\nu}}{\partial x^{\mu}} \cdot \d x^{\mu} \wedge \d x^{\nu}
	\\ \\
	& = &
		\,{\color{white}+}\,
		\left(\,\dfrac{\partial A_{1}}{\partial x^{0}} - \dfrac{\partial A_{0}}{\partial x^{1}}\,\right)\d x^{0} \wedge \d x^{1}
		\,+\,
		\left(\,\dfrac{\partial A_{2}}{\partial x^{0}} - \dfrac{\partial A_{0}}{\partial x^{2}}\,\right)\d x^{0} \wedge \d x^{2}
		\,+\,
		\left(\,\dfrac{\partial A_{3}}{\partial x^{0}} - \dfrac{\partial A_{0}}{\partial x^{3}}\,\right)\d x^{0} \wedge \d x^{3}
	\\
	&&
		\,+\,
		\left(\,\dfrac{\partial A_{2}}{\partial x^{1}} - \dfrac{\partial A_{1}}{\partial x^{2}}\,\right)\d x^{1} \wedge \d x^{2}
		\,+\,
		\left(\,\dfrac{\partial A_{3}}{\partial x^{1}} - \dfrac{\partial A_{1}}{\partial x^{3}}\,\right)\d x^{1} \wedge \d x^{3}
		\,+\,
		\left(\,\dfrac{\partial A_{3}}{\partial x^{2}} - \dfrac{\partial A_{2}}{\partial x^{3}}\,\right)\d x^{2} \wedge \d x^{3}
	\\ \\
	& = &
		\,{\color{white}+}\,
		\left(\,A_{1,0} \overset{{\color{white}.}}{-} A_{0,1}\,\right)
		\d x^{0} \wedge \d x^{1}
		\,+\,
		\left(\,A_{2,0} \overset{{\color{white}.}}{-} A_{0,2}\,\right)
		\d x^{0} \wedge \d x^{2}
		\,+\,
		\left(\,A_{3,0} \overset{{\color{white}.}}{-} A_{0,3}\,\right)
		\d x^{0} \wedge \d x^{3}
	\\
	&&
		\,+\,
		\left(\,A_{2,1} \overset{{\color{white}.}}{-} A_{1,2}\,\right)
		\d x^{1} \wedge \d x^{2}
		\,+\,
		\left(\,A_{3,1} \overset{{\color{white}.}}{-} A_{1,3}\,\right)
		\d x^{1} \wedge \d x^{3}
		\,+\,
		\left(\,A_{3,2} \overset{{\color{white}.}}{-} A_{2,3}\,\right)
		\d x^{2} \wedge \d x^{3}
	\end{eqnarray*}
	Hence,
	\begin{eqnarray*}
	\star\;\d\,\mathbf{A}
	& = &
		\,{\color{white}+}\,
		\left(\,A_{1,0} \overset{{\color{white}.}}{-} A_{0,1}\,\right)
		\cdot
		\star\left(\d x^{0} \wedge \d x^{1}\right)
		\,+\,
		\left(\,A_{2,0} \overset{{\color{white}.}}{-} A_{0,2}\,\right)
		\cdot
		\star\left(\d x^{0} \wedge \d x^{2}\right)
		\,+\,
		\left(\,A_{3,0} \overset{{\color{white}.}}{-} A_{0,3}\,\right)
		\cdot
		\star\left(\d x^{0} \wedge \d x^{3}\right)
	\\
	&&
		\,+\,
		\left(\,A_{2,1} \overset{{\color{white}.}}{-} A_{1,2}\,\right)
		\cdot
		\star\left(\d x^{1} \wedge \d x^{2}\right)
		\,+\,
		\left(\,A_{3,1} \overset{{\color{white}.}}{-} A_{1,3}\,\right)
		\cdot
		\star\left(\d x^{1} \wedge \d x^{3}\right)
		\,+\,
		\left(\,A_{3,2} \overset{{\color{white}.}}{-} A_{2,3}\,\right)
		\cdot
		\star\left(\d x^{2} \wedge \d x^{3}\right)
	\\ \\
	& = &
		\,{\color{white}+}\,
		\left(\,A_{1,0} \overset{{\color{white}.}}{-} A_{0,1}\,\right)
		\d x^{2} \wedge \d x^{3}
		\,+\,
		\left(\,A_{2,0} \overset{{\color{white}.}}{-} A_{0,2}\,\right)
		\d x^{3} \wedge \d x^{1}
		\,+\,
		\left(\,A_{3,0} \overset{{\color{white}.}}{-} A_{0,3}\,\right)
		\d x^{1} \wedge \d x^{2}
	\\
	&&
		\,-\,
		\left(\,A_{2,1} \overset{{\color{white}.}}{-} A_{1,2}\,\right)
		\d x^{0} \wedge \d x^{3}
		\,+\,
		\left(\,A_{3,1} \overset{{\color{white}.}}{-} A_{1,3}\,\right)
		\d x^{0} \wedge \d x^{2}
		\,-\,
		\left(\,A_{3,2} \overset{{\color{white}.}}{-} A_{2,3}\,\right)
		\d x^{0} \wedge \d x^{1}
	\end{eqnarray*}
	Hence,
	\begin{eqnarray*}
	\d\left(\;\star\;\d\,\mathbf{A}\,\right)
	& = &
		\,{\color{white}+}\,
		(\,A_{1,0} \overset{{\color{white}.}}{-} A_{0,1}\,)_{,\,\mu} \cdot \d x^{\mu} \wedge \d x^{2} \wedge \d x^{3}
		\,+\,
		(\,A_{2,0} \overset{{\color{white}.}}{-} A_{0,2}\,)_{,\,\mu} \cdot \d x^{\mu} \wedge \d x^{3} \wedge \d x^{1}
	\\
	&&
		\,+\,
		(\,A_{3,0} \overset{{\color{white}.}}{-} A_{0,3}\,)_{,\,\mu} \cdot \d x^{\mu} \wedge \d x^{1} \wedge \d x^{2}
		\,-\,
		(\,A_{2,1} \overset{{\color{white}.}}{-} A_{1,2}\,)_{,\,\mu} \cdot \d x^{\mu} \wedge \d x^{0} \wedge \d x^{3}
	\\
	&&
		\,+\,
		(\,A_{3,1} \overset{{\color{white}.}}{-} A_{1,3}\,)_{,\,\mu} \cdot \d x^{\mu} \wedge \d x^{0} \wedge \d x^{2}
		\,-\,
		(\,A_{3,2} \overset{{\color{white}.}}{-} A_{2,3}\,)_{,\,\mu} \cdot \d x^{\mu} \wedge \d x^{0} \wedge \d x^{1}
	\\ \\
	& = &
		\,{\color{white}+}\,
		(\,A_{1,00} \overset{{\color{white}.}}{-} A_{0,10}\,) \cdot \d x^{0} \wedge \d x^{2} \wedge \d x^{3}
		\,+\,
		(\,A_{1,01} \overset{{\color{white}.}}{-} A_{0,11}\,) \cdot \d x^{1} \wedge \d x^{2} \wedge \d x^{3}
	\\
	&&
		\,+\,
		(\,A_{2,00} \overset{{\color{white}.}}{-} A_{0,20}\,) \cdot \d x^{0} \wedge \d x^{3} \wedge \d x^{1}
		\,+\,
		(\,A_{2,02} \overset{{\color{white}.}}{-} A_{0,22}\,) \cdot \d x^{2} \wedge \d x^{3} \wedge \d x^{1}
	\\
	&&
		\,+\,
		(\,A_{3,00} \overset{{\color{white}.}}{-} A_{0,30}\,) \cdot \d x^{0} \wedge \d x^{1} \wedge \d x^{2}
		\,+\,
		(\,A_{3,03} \overset{{\color{white}.}}{-} A_{0,33}\,) \cdot \d x^{3} \wedge \d x^{1} \wedge \d x^{2}
	\\
	&&
		\,-\,
		(\,A_{2,11} \overset{{\color{white}.}}{-} A_{1,21}\,) \cdot \d x^{1} \wedge \d x^{0} \wedge \d x^{3}
		\,-\,
		(\,A_{2,12} \overset{{\color{white}.}}{-} A_{1,22}\,) \cdot \d x^{2} \wedge \d x^{0} \wedge \d x^{3}
	\\
	&&
		\,+\,
		(\,A_{3,11} \overset{{\color{white}.}}{-} A_{1,31}\,) \cdot \d x^{1} \wedge \d x^{0} \wedge \d x^{2}
		\,+\,
		(\,A_{3,13} \overset{{\color{white}.}}{-} A_{1,33}\,) \cdot \d x^{3} \wedge \d x^{0} \wedge \d x^{2}
	\\
	&&
		\,-\,
		(\,A_{3,22} \overset{{\color{white}.}}{-} A_{2,32}\,) \cdot \d x^{2} \wedge \d x^{0} \wedge \d x^{1}
		\,-\,
		(\,A_{3,23} \overset{{\color{white}.}}{-} A_{2,33}\,) \cdot \d x^{3} \wedge \d x^{0} \wedge \d x^{1}
	\\ \\
	& = &
		\;{\color{white}+}\;
		\left[\,
			{\color{white}-}
			(\,A_{3,00} \overset{{\color{white}.}}{-} A_{0,30}\,)
			-
			(\,A_{3,11} \overset{{\color{white}.}}{-} A_{1,31}\,) 
			-
			(\,A_{3,22} \overset{{\color{white}.}}{-} A_{2,32}\,)
			\,\right]
			\cdot
			\d x^{0} \wedge \d x^{1} \wedge \d x^{2}
	\\
	&&
		\; + \;
		\left[\,
			- (\,A_{2,00} \overset{{\color{white}.}}{-} A_{0,20}\,)
			+ (\,A_{2,11} \overset{{\color{white}.}}{-} A_{1,21}\,)
			- (\,A_{3,23} \overset{{\color{white}.}}{-} A_{2,33}\,)
			\,\right]
			\cdot
			\d x^{0} \wedge \d x^{1} \wedge \d x^{3}
	\\
	&&
		\; + \;
		\left[\,
			{\color{white}+}
			(\,A_{1,00} \overset{{\color{white}.}}{-} A_{0,10}\,)
			+
			(\,A_{2,12} \overset{{\color{white}.}}{-} A_{1,22}\,)
			+
			(\,A_{3,13} \overset{{\color{white}.}}{-} A_{1,33}\,)
			\,\right]
			\cdot
			\d x^{0} \wedge \d x^{2} \wedge \d x^{3}
	\\
	&&
		\; + \;
		\left[\,
			{\color{white}+}
			(\,A_{1,01} \overset{{\color{white}.}}{-} A_{0,11}\,)
			+
			(\,A_{2,02} \overset{{\color{white}.}}{-} A_{0,22}\,)
			+
			(\,A_{3,03} \overset{{\color{white}.}}{-} A_{0,33}\,)
			\,\right]
			\cdot
			\d x^{1} \wedge \d x^{2} \wedge \d x^{3}
	\end{eqnarray*}
	Hence,
	\begin{eqnarray*}
	\star\;\,\d\left(\;\star\;\d\,\mathbf{A}\,\right)
	& = &
		\;{\color{white}+}\;
		\left[\,
			{\color{white}-}
			(\,A_{3,00} \overset{{\color{white}.}}{-} A_{0,30}\,)
			-
			(\,A_{3,11} \overset{{\color{white}.}}{-} A_{1,31}\,) 
			-
			(\,A_{3,22} \overset{{\color{white}.}}{-} A_{2,32}\,)
			\,\right]
			\cdot
			\;\star\left(\,\d x^{0} \wedge \d x^{1} \wedge \d x^{2}\,\right)
	\\
	&&
		\; + \;
		\left[\,
			- (\,A_{2,00} \overset{{\color{white}.}}{-} A_{0,20}\,)
			+ (\,A_{2,11} \overset{{\color{white}.}}{-} A_{1,21}\,)
			- (\,A_{3,23} \overset{{\color{white}.}}{-} A_{2,33}\,)
			\,\right]
			\cdot
			\;\star\left(\,\d x^{0} \wedge \d x^{1} \wedge \d x^{3}\,\right)
	\\
	&&
		\; + \;
		\left[\,
			{\color{white}+}
			(\,A_{1,00} \overset{{\color{white}.}}{-} A_{0,10}\,)
			+
			(\,A_{2,12} \overset{{\color{white}.}}{-} A_{1,22}\,)
			+
			(\,A_{3,13} \overset{{\color{white}.}}{-} A_{1,33}\,)
			\,\right]
			\cdot
			\;\star\left(\,\d x^{0} \wedge \d x^{2} \wedge \d x^{3}\,\right)
	\\
	&&
		\; + \;
		\left[\,
			{\color{white}+}
			(\,A_{1,01} \overset{{\color{white}.}}{-} A_{0,11}\,)
			+
			(\,A_{2,02} \overset{{\color{white}.}}{-} A_{0,22}\,)
			+
			(\,A_{3,03} \overset{{\color{white}.}}{-} A_{0,33}\,)
			\,\right]
			\cdot
			\;\star\left(\,\d x^{1} \wedge \d x^{2} \wedge \d x^{3}\,\right)
	\\ \\
	& = &
		\; - \;
		\left[\,
			{\color{white}-}
			(\,A_{3,00} \overset{{\color{white}.}}{-} A_{0,30}\,)
			-
			(\,A_{3,11} \overset{{\color{white}.}}{-} A_{1,31}\,) 
			-
			(\,A_{3,22} \overset{{\color{white}.}}{-} A_{2,32}\,)
			\,\right]
			\cdot
			\d x^{3}
	\\
	&&
		\; + \;
		\left[\,
			- (\,A_{2,00} \overset{{\color{white}.}}{-} A_{0,20}\,)
			+ (\,A_{2,11} \overset{{\color{white}.}}{-} A_{1,21}\,)
			- (\,A_{3,23} \overset{{\color{white}.}}{-} A_{2,33}\,)
			\,\right]
			\cdot
			\d x^{2}
	\\
	&&
		\; - \;
		\left[\,
			{\color{white}+}
			(\,A_{1,00} \overset{{\color{white}.}}{-} A_{0,10}\,)
			+
			(\,A_{2,12} \overset{{\color{white}.}}{-} A_{1,22}\,)
			+
			(\,A_{3,13} \overset{{\color{white}.}}{-} A_{1,33}\,)
			\,\right]
			\cdot
			\d x^{1}
	\\
	&&
		\; - \;
		\left[\,
			{\color{white}+}
			(\,A_{1,01} \overset{{\color{white}.}}{-} A_{0,11}\,)
			+
			(\,A_{2,02} \overset{{\color{white}.}}{-} A_{0,22}\,)
			+
			(\,A_{3,03} \overset{{\color{white}.}}{-} A_{0,33}\,)
			\,\right]
			\cdot
			\d x^{0}
	\\ \\
	& = &
		\; - \;
		\left[\,
			{\color{white}+}\,
			(\,A_{3,00} \overset{{\color{white}.}}{-} A_{3,11}  - A_{3,22} \,{\color{red}- A_{3,33}}\,)
			+
			(\,-\,A_{0,03} \overset{{\color{white}.}}{+} A_{1,13} + A_{2,23} \,{\color{red}+A_{3,33}}\,)
			\,\right]
			\cdot
			\d x^{3}
	\\
	&&
		\; + \;
		\left[\,
			-\,
			(\,A_{2,00} \overset{{\color{white}.}}{-} A_{2,11} \,{\color{red}- A_{2,22}} - A_{2,33}\,)
			-
			(\,-\,A_{0,02} \overset{{\color{white}.}}{+} A_{1,12} \,{\color{red}+A_{2,22}} + A_{3,32}\,)
			\,\right]
			\cdot
			\d x^{2}
	\\
	&&
		\; - \;
		\left[\,
			{\color{white}+}\,
			(\,A_{1,00} \,{\color{red}- A_{1,11}} \overset{{\color{white}.}}{-} A_{1,22} - A_{1,33}\,)
			+
			(\,-\,A_{0,01} \,{\color{red}+ A_{1,11}} \overset{{\color{white}.}}{+} A_{2,21} + A_{3,31}\,)
			\,\right]
			\cdot
			\d x^{1}
	\\
	&&
		\; - \;
		\left[\,
			\overset{{\color{white}.}}{-}\,
			(\,A_{0,11} + A_{0,22} + A_{0,33}\,)
			\,+\,
			(\,A_{1,10} + A_{2,20} + A_{3,30}\,)
			\,\right]
			\cdot
			\d x^{0}
	\\ \\
	& = &
		\; - \;
		\left[\,
			\left(\,\dfrac{\partial^{2}}{\partial(x^{0})^{2}} - \Delta\,\right)A
			+
			\nabla\left(\, -\,\dfrac{\partial A_{0}}{\partial x^{0}} + \nabla \bullet A \,\right)
			\,\right]_{3}
			\cdot
			\d x^{3}
	\\
	&&
		\; - \;
		\left[\,
			\left(\,\dfrac{\partial^{2}}{\partial(x^{0})^{2}} - \Delta\,\right)A
			+
			\nabla\left(\, -\,\dfrac{\partial A_{0}}{\partial x^{0}} + \nabla \bullet A \,\right)
			\,\right]_{2}
			\cdot
			\d x^{2}
	\\
	&&
		\; - \;
		\left[\,
			\left(\,\dfrac{\partial^{2}}{\partial(x^{0})^{2}} - \Delta\,\right)A
			+
			\nabla\left(\, -\,\dfrac{\partial A_{0}}{\partial x^{0}} + \nabla \bullet A \,\right)
			\,\right]_{1}
			\cdot
			\d x^{1}
	\\
	&&
		\; - \;
		\left[\,
			-\,\Delta A_{0} + \dfrac{\partial}{\partial x^{0}}\!\left(\,\nabla \bullet A\,\right)
			\,\right]
			\cdot
			\d x^{0}
	\end{eqnarray*}
	Hence, we see that
	\begin{equation*}
	\textnormal{$B$\, and \,$E$\, satisfy Gauss's law for electric fields and Amp\`{e}re-Maxwell's law}
	\end{equation*}
	if and only if
	\begin{eqnarray*}
	\star\;\,\d\left(\;\star\;\mathbf{F}\,\right)
	& = &
		4\,\pi \cdot \mathbf{J}
	\end{eqnarray*}
	if and only if
	\begin{eqnarray*}
	\star\;\,\d\left(\;\star\;\d\mathbf{A}\,\right)
	& = &
		4\,\pi \cdot \left(\,\rho\,\d x^{0} - J^{1}\,\d x^{1} - J^{2}\,\d x^{2} - J^{3}\,\d x^{3}\,\right)
	\end{eqnarray*}
	if and only if
	\begin{equation*}
	\left\{\begin{array}{ccl}
		-\,\Delta A_{0} + \dfrac{\partial}{\partial x^{0}}\!\left(\,\nabla \bullet A\,\right)
		& = &
			- \, 4\,\pi\cdot\rho
		\\ \\
		\left(\,\dfrac{\partial^{2}}{\partial(x^{0})^{2}} - \Delta\,\right)A
		+
		\nabla\left(\, -\,\dfrac{\partial A_{0}}{\partial x^{0}} + \nabla \bullet A \,\right)
		& = &
			{\color{white}-} \, 4\,\pi \cdot J
		\end{array}\right.
	\end{equation*}
	as required.
\end{enumerate}
\vskip 0.3cm
The proof of the Theorem is complete.
\qed

          %%%%% ~~~~~~~~~~~~~~~~~~~~ %%%%%

          %%%%% ~~~~~~~~~~~~~~~~~~~~ %%%%%

          %%%%% ~~~~~~~~~~~~~~~~~~~~ %%%%%

          %%%%% ~~~~~~~~~~~~~~~~~~~~ %%%%%

          %%%%% ~~~~~~~~~~~~~~~~~~~~ %%%%%

